functional code

Homework6.dfy
@@ -3,27 +3,66 @@ datatype List<T> = Nil | Cons(T, List<T>)
 
 function flatten<T>(tree:Tree<T>):List<T>
 {
-	
+	match tree
+    case Leaf => Nil
+    case Node(left, right, ele) => append(flatten(left), append(flatten(right), Cons(ele, Nil)))
 }
 
+
 function append<T>(xs:List<T>, ys:List<T>):List<T>
+ensures xs == Nil ==> append(xs, ys) == ys
+ensures ys == Nil ==> append(xs, ys) == xs
+ensures length(append(xs,ys)) == length(xs) + length(ys)
 {
-	
+    match xs
+    case Nil => ys
+    case Cons(x,xs') => Cons(x, append(xs',ys))
 }
+
+
+function length<T>(xs:List<T>) : int
+{
+    match xs
+    case Nil => 0
+    case Cons(x,xs') => 1 + length(xs')
+}
+
 
 function treeContains<T>(tree:Tree<T>, element:T):bool
 {
-	
+	match tree
+    // case Leaf => (Leaf == element) || false
+    case Leaf => false
+    case Node(left, right, val) => treeContains(left, element) || treeContains(right, element) || (val == element)
 }
+
 
 function listContains<T>(xs:List<T>, element:T):bool
 {
-	
-}
+	match xs
+    case Nil => false
+    case Cons(x, xs') => (x==element) || listContains(xs', element)
+}   
 
 
 lemma sameElements<T>(tree:Tree<T>, element:T)
 ensures treeContains(tree, element) <==> listContains(flatten(tree), element)
-{
+{   
+    // match(tree)
+    // case Leaf => {}
+    // case Node(left, right, ele) => {
+    //     calc { treeContains(tree, element) ;
+    //         == treeContains(Node(left, right, ele), element) ;
+    //         == treeContains(left, element) || treeContains(right, element) || (ele == element) ;
+    //         == listContains(flatten(left), element) || listContains(flatten(right), element) || (ele == element) ;
+            
+    //         == listContains(flatten(left), element) || listContains(flatten(right), element) || listContains(Cons(ele, Nil), element) ;
+    //         == listContains(flatten(left), element) || listContains(append(flatten(right), Cons(ele, Nil)), element) ;
+    //         == listContains(append(flatten(left), append(flatten(right), Cons(ele, Nil))), element) ;
+    //         == listContains(flatten(tree), element) ;
+
+        
+    //     }
+    // }
 	
 }
